## exercise 1.10

``` Scheme
#lang racket

(define (A x y)
  (cond ((= y 0) 0)
        ((= x 0) (* 2 y))
        ((= y 1) 2)
        (else (A (- x 1)
                 (A x (- y 1))))))

(A 1 10)
(A 2 4)
(A 3 3)
```

we can know

```
(A 1 10) = 1024
(A 2 4) = 65536
(A 3 3) = 65536
```

---------

we can also expand the calculation process manually.

``` Scheme
(A 1 10)
(A 0 (A 1 9))
(* 2 (A 1 9))
(* 2 (A 0 (A 1 8))
(* 2 (* 2 (A 1 8))
(* 2 (* 2 (A 0 (A 1, 7))
(* 2 (* 2 (* 2 (A 1, 7))
....
(* 2 (* 2 (* 2 (* 2 ....(* 2 (A 1 1))))))))))
(* 2 (* 2 (* 2 (* 2 ....(* 2 2)))))))       ;;Multiply ten twos in a row
....
1024
```

As can be seen from the expansion of `(A 1 10)` , the result of (A 1 n) is the multiplication of n 2, that is, 2 to the power of n `(expt 2 n)`

``` Scheme
(A 2 4)
(A 1 (A 2 3))
(A 1 (A 1 (A 1 2)))
;;Then, instead of expanding gradually, we use the conclusion (A 1 n) = (expt 2 n).
...
(A 1 (A 1 4))
(A 1 16)
65536
```

t can be seen from the expansion process of `(A 2 4)` that the result of (A 2 n) is continuously raised to the NTH power.That is, `(expt 2 (expt 2 (expt 2 1)))`, that is

``` Scheme
(A 2 1) = (expt 2 1) = 2
(A 2 2) = (expt 2 (A 2 1)) = (expt 2 2) = 4
(A 2 3) = (expt 2 (A 2 2)) = (expt 2 4) = 16
(A 2 4) = (expt 2 (A 2 3)) = (expt 2 16) = 65536
(A 2 5) = (expt 2 (A 2 4)) = (expt 2 65536) = 超级大的数字
```

``` Scheme
(A 3 3)
(A 2 (A 3 2))
(A 2 (A 2 (A 3 1)))
(A 2 (A 2 2))
;; 接下来直接应用 (A 2 n) 的展开结果，为
(A 2 4)
65536
```

---------

You can use the program to print out the previous values and summarize the formula.Or expand the analysis manually.

* (A 0 n) is expanded to (* 2 n), and the mathematical formula is 2 * n
* (A 1 n), as I said up here, is 2 to the n, expt 2 n.The mathematical formula is 2 to the n.
* (A 2 n) which I said up here, to the NTH power.The mathematical formula is 2 ^ (2 ^ (2 ^...)(2 ^ 2)) 'n times.

Use the program to print out the numbers and table them

 n       | 0  | 1  | 2  | 3   | 4     | 5   | 6   | 7   | 8   | ... |
---------|----|----|----|-----|-------|-----|-----|-----|-----|-----|
 (A 0 n) | 0  | 2  | 4  | 6   | 8     | 10  | 12  | 14  | 16  | ... |
 (A 1 n) | 0  | 2  | 4  | 8   | 16    | 32  | 64  | 128 | 256 | ... |
 (A 2 n) | 0  | 2  | 4  | 16  | 65536 | ... | ... | ... | ... | ... |


---------

The formula can also be derived according to mathematical induction:

``` Scheme
(f n) =
(A 0 n) =
(* 2 n)
;;So (f n) is 2n
```

``` Scheme
(g n) =
(A 1 n) =
(A 0 (A 1 (- n 1))) =
(f (A 1 (- n 1))) =
(f (g (- n 1))) =
(* 2 (g (- n 1)))
;;So  g(n) = 2 * g(n - 1)
;;And g(1) = 2
;;We can prove by induction that (g n) = 2 ^ n
```

``` Scheme
(h n) =
(A 2 n) =
(A 1 (A 2 (- n 1))) =
(g (A 2 (- n 1))) =
(g (h (- n 1))) =
(expt 2 (h (- n 1)))
;; So h(n) = 2 ^ h(n - 1)
;; and h(1) = 2
;; It can be proved by induction that (h n) = 2 ^ (2 ^ (2 ^ ... (2 ^ 2)))
```
