## exercise 5.29

Execute the following code using the [evaluator](./ch5-eceval.scm).

``` Scheme
(define (fib n)
  (if (< n 2)
      n
      (+ (fib (- n 1)) (fib (- n 2)))))

(fib 2)   ; (total-pushes = 72 maximum-depth = 13)
(fib 3)   ; (total-pushes = 128 maximum-depth = 18)
(fib 4)   ; (total-pushes = 240 maximum-depth = 23)
(fib 5)   ; (total-pushes = 408 maximum-depth = 28)
(fib 6)   ; (total-pushes = 688 maximum-depth = 33)
(fib 7)   ; (total-pushes = 1136 maximum-depth = 38)
(fib 8)   ; (total-pushes = 1864 maximum-depth = 43) 
(fib 9)   ; (total-pushes = 3040 maximum-depth = 48)
(fib 10)  ; (total-pushes = 4944 maximum-depth = 53)
```

Gets information about `total-pushes` and `maximum-depth`.

Make a table.To facilitate answer b, line 3 also lists Fibonacci's results.

|  n               | 2  | 3  | 4  | 5  | 6  | 7  | 8  | 9  | 10 |
|--------------    |----|----|----|----|----|----|----|----|----|
| maximum-depth    | 13 | 18 | 23 | 28 | 33 | 38 | 43 | 48 | 53 |
| total-pushes     | 72 | 128| 240| 408| 688|1136|1864|3040|4944|
| Fib(n)           | 1  | 2  | 3  | 5  | 8  | 13 | 21 | 34 | 55 |

### a)

As can be seen from the table, the value of maximum-depth is an arithmetic sequence. The difference between the two terms is 5, which can be calculated

```
maximum-depth = 13 + (n - 2) * 5 = 5 * n + 3
```

where n >= 2。

### b)

To make this easier, we use S(n) to denote `total-pushes`，where n >= 2. So there is

```
S(2) = 72
S(3) = 128
S(4) = 240
S(5) = 408
S(6) = 688
....
```

Based on the numbers above, we can figure out

```
S(n) = S(n - 1) + S(n - 2) + 40 ; n >= 4
```

Compare the values of S(n) and Fib(n+1)

|  n       | 2  | 3  | 4  | 5  | 6  | 7  | 8  | 9  |
|--------- |----|----|----|----|----|----|----|----|
| S(n)     | 72 | 128| 240| 408| 688|1136|1864|3040|
| Fib(n+1) | 2  | 3  | 5  | 8  | 13 | 21 | 34 | 55 |

And according to the problem, this is a linear relationship.Let me write an equation. We can figure it out

```
S(n) = 56 * Fib(n+1) - 40 ; n >= 2
```

### c)

Now let's prove the linear relationship between `S(n)` 和 `Fib(n+1)` in b).Mathematical induction is adopted.

First of all, when n = 2 and n = 3, in the base case, this relationship is true.

```
S(2) = 56 * Fib(3) - 40 = 56 * 2 - 40 = 72
S(3) = 56 * Fib(4) - 40 = 56 * 3 - 40 = 128
```

So in the recursive case, I have

```
S(n) = S(n - 1) + S(n - 2) + 40
=> S(n) = [56 * Fib(n) - 40] + [56 * Fib(n - 1) - 40] + 40
=> S(n) = 56 * [Fib(n) + Fib(n - 1)] - 40
=> S(n) = 56 * Fib(n+1) - 40
```

So, in the recursive case, the relationship holds.So this is a linear relationship.

```
S(n) = 56 * Fib(n+1) - 40 ; n >= 2
```
