## exercise 3.57

``` Scheme
(define fibs 
  (cons-stream 0
               (cons-stream 1
                            (add-streams (stream-cdr fibs) 
                                         fibs))))
```                                        

According to the fibs definition, to compute the NTH number, you need to compute the n-1 and n-2 values first.There are

```
(stream-ref fibs 0) = 0                                        
(stream-ref fibs 1) = 1                                        
(stream-ref fibs 2) = (stream-ref fibs 1) + (stream-ref fibs 0)
(stream-ref fibs 3) = (stream-ref fibs 2) + (stream-ref fibs 1)
(stream-ref fibs 4) = (stream-ref fibs 3) + (stream-ref fibs 2)
...
(stream-ref fibs n) = (stream-ref fibs (- n 1)) + (stream-ref fibs (- n 2))
```

### a)

For delay with memory, for each i, `(stream-ref fibs i)`will be evaluated only once, and the result will be returned directly if evaluated again.So the NTH Fibonacci number is only one more addition than the n-1 number.The number of additions needed to calculate the NTH number (number starting from 0) is denoted as A(n), while the 0 and 1 numbers are given directly without addition.So there is

```
A(0) = 0
A(1) = 0
A(2) = 1
A(3) = 2
A(4) = 3
....
A(n) = n - 1
```

### b)

There is no memory delay, and for each i, `(stream-ref fibs i)` is re-evaluated each time it is called
```
(stream-ref fibs n) = (stream-ref fibs (- n 1)) + (stream-ref fibs (- n 2))
```

Then the number of additions you need, A(n), will be there

```
A(0) = 0
A(1) = 0
A(2) = A(1) + A(0) + 1 = 1
...
A(n) = A(n - 1) + A(n - 2) + 1 ; You need to add up the first two fib numbers, so you need to add an extra 1
```

Notice that the recursive formula at the end is very similar to the definition of Fibs, but with an extra 1.Compare this to the formal Fib definition

```
Fib(0) = 0
Fib(1) = 1
Fib(2) = Fib(1) + Fib(0) = 1
...
Fib(n) = Fib(n - 1) + Fib(n - 2)
```

Make a list

```
n   0   1   2   3   4   5   6   7   8   9   10  11  12
--------------------------------------------------------
A   0   0   1   2   4   7   12  20  33  54  88  143 --
Fib 0   1   1   2   3   5   8   13  21  34  55  89  144
```

A reasonable guess can be made from the table

```
A(n) = Fib(n + 1) - 1	; n >= 0
```

Prove the above formula by mathematical induction.

```
A(0) = 0, Fib(1) - 1 = 0
A(1) = 0, Fib(2) - 1 = 0
```

Obviously in the base case the formula works.So let's say this is true for n, for n plus 1, there's

```
A(n + 1) = A(n) + A(n - 1) + 1
         = Fib(n + 1) - 1 + Fib(n) - 1 + 1
         = Fib(n + 1) + Fib(n) - 1
         = Fib(n + 2) - 1
```

And we know that the recursion is also true.The original formula is proved.

See exercise 1.13 proof,  `Fib(n)`  is the most close to $\frac{\phi^{n}}{\sqrt{5}}$ integer.That's the exponential growth of n.

So the addition required to compute the Nth Fibonacci number without memorization is

```
A(n) = Fib(n + 1) - 1
```

It's also exponential growth in n.
